\documentclass[11pt]{article}

\usepackage{amssymb}
\usepackage{amsmath}
\usepackage{amsthm}
\usepackage{indentfirst}
\usepackage{amsmath, array}
\usepackage{graphics}

\title{Section 8.5 Notes}

\begin{document}
\maketitle

\section*{8.5.2}

Expand the quotient by partial fractions:

$$\frac{5x-7}{x^2-3x+2} = \frac{5x-7}{(x-2)(x-1)}$$

Before doing anything else, check that the degree of the numerator is strictly less than the degree of the denominator. Otherwise you'll end up doing a lot of algebra only to find out that partial fractions 'breaks'...yes the degree of the numerator is 1 and the degree of the denominator is 2. 


$$\frac{5x-7}{(x-2)(x-1)} = \frac{A}{x-2} + \frac{B}{x-1}$$
$$5x-7 = A(x-1) + B(x-2)$$
$$5x-7 = (A+B)x + (-A-2B)$$
Matching the $'x'$ coefficients on both sides and matching the constants on both sides gives two equations:
$$5 = A+B \quad -7 = -A-2B$$
Solve this system of equations however you prefer. The result is 
$A = 3, B= 2$. Conclude that:

$$\frac{5x-7}{(x-2)(x-1)} = \frac{A}{x-2} + \frac{B}{x-1} = \frac{3}{x-2} + \frac{2}{x-1}$$

This means that if we were asked to evaluate $\int \frac{5x-7}{(x-2)(x-1)} \, dx$, it would be the same thing as evaluate $\int (\frac{3}{x-2} + \frac{2}{x-1}) \, dx$. The second integral is easier to find. 

\section*{8.5.8}

Expand the quotient by partial fractions:

$$\frac{t^4+9}{t^4+9t^2}$$

The degree of the numerator is not less than the degree of the denominator, so first long division:


\begin{align*}                                                                      
  \renewcommand\arraystretch{2}                                                     
  \begin{array}{r@{\hskip\arraycolsep}c@{\hskip\arraycolsep}l*2r}                   
    &&1\\[.1cm]                                                                      
    \cline{2-3}                                                                     
    t^4+9t^2 &\Bigg)&t^4+9\\[.1cm]                     
    &&-(t^4+9t^2)\\[.1cm]                           
    \cline{2-3}                                                                     
    &&\hfill-9t^2+9\\[.1cm]                                                         
  \end{array}                                                                       
\end{align*}

$$\frac{t^4+9}{t^4+9t^2} = 1 + \frac{-9t^2+9}{t^4+9t^2} = 1 + \frac{-9t^2+9}{t^2(t^2+9)}$$

Just work with the fraction part for now.

$$ \frac{-9t^2+9}{t^2(t^2+9)} = \frac{A}{t} + \frac{B}{t^2} + 
\frac{Ct + D}{t^2+9}$$
$$-9t^2 + 9 = At(t^2+9) + B(t^2+9) + (Ct+D)t^2$$

$$-9t^2 + 9 = (A+C)t^3 + (B+D)t^2 + (9A)t + 9B$$

Equating coefficients gives the four equations:

$$0 = A+C$$
$$-9 = B+D$$
$$0 = A$$
$$9 = 9B$$

This system has the solution $A = 0, B = 1, C = 0, D = -10$. Conclude that 
$$\frac{t^4+9}{t^4+9t^2} = 1 + \frac{-9t^2+9}{t^2(t^2+9)} = \frac{A}{t} + \frac{B}{t^2} + 
\frac{Ct + D}{t^2+9} = 1 + \frac{1}{t^2} - \frac{10}{t^2+9}$$

\end{document}