\documentclass[11pt]{article}

\usepackage{amssymb}
\usepackage{amsmath}
\usepackage{amsthm}
\usepackage{indentfirst}

\title{Section 8.3 Notes}

\begin{document}
\maketitle

\section*{8.3.4}

\begin{align*}
&\int \text{sin}^4(2x)\text{cos}(2x) \, dx\\
&u = \text{sin}(2x) \quad du = 2\text{cos}(2x) dx\\
&=\frac{1}{2}\int u^4 \, du\\
&=\frac{1}{10}u^5 + C\\
&=\frac{1}{10}\text{sin}^5(2x) + C
\end{align*}

\section*{8.3.5}

\begin{align*}
&\int \text{sin}^3(x) \, dx\\
&=\int (1-\text{cos}^2(x))\text{sin}(x) \, dx\\
&u = \text{cos}(x) \quad du = -\text{sin}(x) dx\\
&=-\int (1-u^2)\, du\\
&= \frac{1}{3}u^3 - u + C\\
&=\frac{1}{3}\text{cos}^3(x)-\text{cos}(x) + C
\end{align*}

\section*{8.3.27 (Most of the Work)}

\begin{align*}
&\int_{\pi/3}^{\pi/2} \frac{\text{sin}^2(x) \, dx}{\sqrt{1-\text{cos}(x)}} \\
&=\int_{\pi/3}^{\pi/2} \frac{\text{sin}^2(x)\sqrt{1+\text{cos}(x)} \, dx}{\sqrt{1-\text{cos}(x)}\sqrt{1+\text{cos}(x)}} \\
&=\int_{\pi/3}^{\pi/2} \frac{\text{sin}^2(x)\sqrt{1+\text{cos}(x)} \, dx}{\sqrt{(1-\text{cos}(x))(1+\text{cos}(x))}} \\
&=\int_{\pi/3}^{\pi/2} \frac{\text{sin}^2(x)\sqrt{1+\text{cos}(x)} \, dx}{\sqrt{1-\text{cos}^2(x)}} \\
&=\int_{\pi/3}^{\pi/2} \frac{\text{sin}^2(x)\sqrt{1+\text{cos}(x)} \, dx}{\sqrt{\text{sin}^2(x)}} \\
&=\int_{\pi/3}^{\pi/2} \frac{\text{sin}^2(x)\sqrt{1+\text{cos}(x)} \, dx}{|\text{sin}(x)|} \\
&=\int_{\pi/3}^{\pi/2} \frac{\text{sin}^2(x)\sqrt{1+\text{cos}(x)} \, dx}{\text{sin}(x)} \quad (\text{Because sin}(x) > 0 \text{ for } \pi/3\leq x \leq \pi/2)\\
&=\int_{\pi/3}^{\pi/2} \text{sin}(x)\sqrt{1+\text{cos}(x)} \, dx \\
&u = 1+\text{cos}(x) \quad du = -\text{sin}(x) dx\\
&u(\pi/3) = \frac{3}{2} \quad u(\pi/2) = 1\\
&=-\int_{3/2}^{1} \sqrt{u} \, du\\
&...\\
&=-\frac{2}{3} + \sqrt{\frac{3}{2}}
\end{align*}

\end{document}